Example_Parnas_Functional_Decomposition_Changeable.v
@@ -1,0 +1,12 @@
+Require Export Quality.
+Require Export Value.
+Require Export Example_Parnas_Functional_Decomposition.
+Require Export BoehmTactics.
+
+Definition corpusChangeActionSpec (trigger: kwicAssertion) (agent: kwicStakeholders) (pre post: kwicSystemState): Prop  :=  
+        isModular_wrt corpus pre /\ (trigger = corpusPreState /\ agent = customer /\ corpusPre pre /\ inMaintenancePhase pre ->
+        corpusPost post /\ modulesChanged (value post) <= modulesChanged (value pre) + 1).
+
+Theorem verifyChangeCorpus: ActionSatisfiesActionSpec (corpusChangeActionSpec corpusPre customer) costomerChangeCorpus.
+Proof.
+(* Should not be proved *)
