Example_Parnas_Shared_Info.v
@@ -1,0 +1,41 @@
+(** ** Context *)
+
+Inductive kwicContexts := nominal.
+
+(** ** Phase *)
+
+(**
+[kwicPhases] represents the lifecycle phases of a software system.
+*)
+
+(** design, implementation and maintenance are talked about in the paper*)
+Inductive kwicPhases := design | implementation | maintenance.
+
+(** ** Stakeholder *)
+
+(**
+[kwicStakeholders] represents the set of potential system change agents
+*)
+
+Inductive kwicStakeholders :=  developer | customer.
+
+(** ** Value for measuring cost-benefit *)
+
+(** 
+[kwicValue] is a framework for quantifying time, money, and other
+elements of value that can be gained or lost as a result of a change.
+*)
+
+Inductive kwicValue := mk_value { 
+  modulesChanged: nat
+}.
+
+Inductive computerState := computer_pre | computer_post.
+Inductive corpusState := corpus_pre | corpus_post.
+Inductive userState := user_pre | user_post.
+
+Record kwicVolatileState : Set := {
+  computer_state: computerState;
+  corpus_state: corpusState;
+  user_state: userState
+}.
